theories/Substitution/Properties.v
@@ -1,0 +1,150 @@
+From LogRel.AutoSubst Require Import core unscoped Ast.
+From LogRel Require Import Utils BasicAst Notations Context Untyped Weakening GenericTyping LogicalRelation Reduction Irrelevance Escape Reflexivity Validity.
+From LogRel.Substitution Require Import Irrelevance.
+
+Section Properties.
+Context `{GenericTypingProperties}.
+
+
+Lemma wellformedSubst {Γ σ Δ} (VΓ : [||-v Γ]) (wfΔ : [|- Δ]) :
+  [Δ ||-v σ : Γ | VΓ| wfΔ] -> [Δ |-s σ : Γ ].
+Proof.
+  revert σ; pattern Γ, VΓ; apply validity_rect; clear Γ VΓ.
+  - intros. apply well_sempty.
+  - intros * ih σ [tl hd]. 
+    eapply well_scons.
+    + now apply ih.
+    + eapply escapeTerm; [apply (validTy VA wfΔ tl) | exact hd].
+Qed.
+
+Lemma wellformedSubstEq {Γ σ σ' Δ} (VΓ : [||-v Γ]) (wfΔ : [|- Δ]) (Vσ : [Δ ||-v σ : Γ | VΓ | wfΔ]) :
+  [Δ ||-v σ ≅ σ' : Γ | VΓ | wfΔ | Vσ] -> [Δ |-s σ ≅ σ' : Γ].
+Proof.
+  revert σ σ' Vσ; pattern Γ, VΓ; apply validity_rect; clear Γ VΓ.
+  - intros. apply conv_sempty.
+  - intros * ih ??? [tl hd]. apply conv_scons.
+    + now eapply ih.
+    + eapply escapeEqTerm; [eapply (validTy VA wfΔ) | exact hd].
+Qed.
+
+Lemma consSubstS {Γ σ t l nA A Δ} (VΓ : [||-v Γ]) (wfΔ : [|- Δ])
+  (Vσ : [Δ ||-v σ : Γ | VΓ | wfΔ]) (VA : [Γ ||-v<l> A | VΓ])
+  (Vt : [ Δ ||-<l> t : A[σ] | validTy VA wfΔ Vσ]) :
+  [Δ ||-v (t .: σ) : Γ ,, vass nA A | validSnoc nA VΓ VA | wfΔ].
+Proof.  unshelve econstructor; eassumption. Defined.
+
+Lemma consSubstSEq {Γ σ σ' t l nA A Δ} (VΓ : [||-v Γ]) (wfΔ : [|- Δ])
+  (Vσ : [Δ ||-v σ : Γ | VΓ | wfΔ]) 
+  (Vσσ' : [Δ ||-v σ ≅ σ' : Γ | VΓ | wfΔ | Vσ])
+  (VA : [Γ ||-v<l> A | VΓ])
+  (Vt : [Δ ||-<l> t : A[σ] | validTy VA wfΔ Vσ]) :
+  [Δ ||-v (t .: σ) ≅  (t .: σ') : Γ ,, vass nA A | validSnoc nA VΓ VA | wfΔ | consSubstS VΓ wfΔ Vσ VA Vt].
+Proof.
+  unshelve econstructor. 
+  1: eassumption.
+  eapply LRTmEqRefl; [apply (validTy VA wfΔ)| exact Vt].
+Qed.
+
+
+Lemma wkSubstS {Γ} (VΓ : [||-v Γ]) : 
+  forall {σ  Δ Δ'}  (wfΔ : [|- Δ]) (wfΔ' : [|- Δ']) (ρ : Δ ≤ Δ'),
+  [Δ ||-v σ : Γ | VΓ | wfΔ] -> [Δ' ||-v σ ⟨ ρ ⟩ : Γ | VΓ | wfΔ'].
+Proof.
+  pattern Γ, VΓ; apply validity_rect; clear Γ VΓ.
+  - constructor.
+  - intros * ih * [tl hd]; unshelve econstructor.
+    + eapply ih; eassumption.
+    + admit.
+Admitted.
+
+
+Lemma wkSubstSEq {Γ} (VΓ : [||-v Γ]) : 
+  forall {σ σ' Δ Δ'}  (wfΔ : [|- Δ]) (wfΔ' : [|- Δ']) (ρ : Δ ≤ Δ')
+  (Vσ : [Δ ||-v σ : Γ | VΓ | wfΔ]),
+  [Δ  ||-v σ ≅ σ' : Γ | VΓ | wfΔ | Vσ] -> 
+  [Δ' ||-v σ ⟨ ρ ⟩ ≅ σ' ⟨ ρ ⟩ : Γ | VΓ | wfΔ' | wkSubstS VΓ wfΔ wfΔ' ρ Vσ].
+Proof.
+  pattern Γ, VΓ; apply validity_rect; clear Γ VΓ.
+  - constructor.
+  - intros * ih * [tl hd]; unshelve econstructor.
+    + admit. (* eapply ih; eassumption. *)
+    + admit.
+Admitted.
+
+Lemma wk1SubstS {Γ σ Δ nF F} (VΓ : [||-v Γ]) (wfΔ : [|- Δ]) (wfF : [Δ |- F]) :
+  [Δ ||-v σ : Γ | VΓ | wfΔ ] ->
+  [Δ ,, vass nF F ||-v σ ⟨ @wk1 Γ nF F ⟩ : Γ | VΓ | wfc_cons nF wfΔ wfF].
+Proof.
+Admitted.
+
+Lemma wk1SubstSEq {Γ σ σ' Δ nF F} (VΓ : [||-v Γ])
+  (wfΔ : [|- Δ]) (wfF : [Δ |- F])
+  (Vσ : [Δ ||-v σ : Γ | VΓ | wfΔ ]) :
+  [Δ ||-v σ ≅ σ' : Γ | VΓ | wfΔ | Vσ] ->
+  let ρ := @wk1 Γ nF F in
+  [Δ ,, vass nF F ||-v σ ⟨ ρ ⟩ ≅ σ ⟨ ρ ⟩ : Γ | VΓ | wfc_cons nF wfΔ wfF | wk1SubstS VΓ wfΔ wfF Vσ].
+Proof.
+Admitted.
+
+Lemma liftSubstS {Γ σ Δ lF nF F} (VΓ : [||-v Γ]) (wfΔ : [|- Δ])
+  (VF : [Γ ||-v<lF> F | VΓ])
+  (Vσ : [Δ ||-v σ : Γ | VΓ | wfΔ ]) :
+  let VΓF := validSnoc nF VΓ VF in 
+  let ρ := wk_up nF F (@wk_id Γ) in
+  let wfΔF := wfc_cons nF wfΔ (escape_ (validTy VF wfΔ Vσ)) in
+  [Δ ,, vass nF F[σ] ||-v σ ⟨ ρ ⟩ : Γ ,, vass nF F | VΓF | wfΔF ].
+Proof.
+Admitted.
+
+Lemma liftSubstSEq {Γ σ σ' Δ lF nF F} (VΓ : [||-v Γ]) (wfΔ : [|- Δ])
+  (VF : [Γ ||-v<lF> F | VΓ])
+  (Vσ : [Δ ||-v σ : Γ | VΓ | wfΔ ]) :
+  let VΓF := validSnoc nF VΓ VF in 
+  let ρ := wk_up nF F (@wk_id Γ) in
+  let wfΔF := wfc_cons nF wfΔ (escape_ (validTy VF wfΔ Vσ)) in
+  let Vliftσ := liftSubstS VΓ wfΔ VF Vσ in
+  [Δ ||-v σ ≅ σ' : Γ | VΓ | wfΔ | Vσ] ->
+  [Δ ,, vass nF F[σ] ||-v σ ⟨ ρ ⟩ ≅ σ' ⟨ ρ ⟩ : Γ ,, vass nF F | VΓF | wfΔF | Vliftσ].
+Proof.
+Admitted.
+
+Set Printing Primitive Projection Parameters.
+
+Lemma wk1ValidTy {Γ lA A lF nF F} (VΓ : [||-v Γ]) (VF : [Γ ||-v<lF> F | VΓ]) :
+  [Γ ||-v<lA> A | VΓ] -> 
+  [Γ ,, vass nF F ||-v<lA> A ⟨ @wk1 Γ nF F ⟩ | validSnoc nF VΓ VF ].
+Proof.
+  assert (forall σ, (A ⟨@wk1 Γ nF F⟩)[σ] = A[↑ >> σ]) as h by (intros; asimpl; now rewrite wk1_ren) ;
+  intros [VA VAext]; unshelve econstructor.
+  - abstract (intros * [tl _]; rewrite h; exact (VA _ _ wfΔ tl)).
+  - intros * [tl _] [tleq _].
+    rewrite (h σ'); unshelve eapply LRTyEqSym.
+    2: eapply VA; eassumption.
+    rewrite (h σ).
+    eapply VAext. 1: exact (validTail vσ).
+    eapply symmetrySubstEq. eassumption.
+Qed.    
+
+Lemma soundCtxId {Γ} (VΓ : [||-v Γ]) :
+  ∑ wfΓ : [|- Γ], [Γ ||-v tRel : Γ | VΓ | wfΓ].
+Proof.
+  pattern Γ, VΓ; apply validity_rect; clear Γ VΓ.
+  - unshelve econstructor. 1: apply wfc_nil. constructor.
+  - intros * [wfΓ idΓ]. unshelve econstructor.
+    + apply wfc_cons. 1: assumption. eapply escape.  
+      assert (A[tRel] = A) as <- by now asimpl.  
+      apply (validTy VA wfΓ idΓ).
+    + admit.
+    (* unshelve eapply consSubstS.
+      5:{ unshelve econstructor. }
+    replace tRel with (tRel 0 .: S >> tRel). *)
+Admitted.
+ 
+
+
+End Properties.
+
+
+ 
+
+
